part C done

code/UMap.dfy
@@ -4,7 +4,7 @@
 
   Mini Project 3 - Part C
 
-  Your name(s): Example solution
+  Your name(s): Shweta Rajiv and Sage Binder
   ===============================================*/
 
 include "Option.dfy"
@@ -15,46 +15,109 @@ import opened M = Map
 import opened Option
 
 class UMap<T(!new,==)> {
+  var entries: Map<T>
 
   // this.entrySet() is the set of all the entries in the map 
   ghost function entrySet(): set<Entry<T>>
+    reads this
+  {
+    M.entries(entries)
+  }
 
   // this.keySet() is the set of all the keys in the map 
   ghost function keySet(): set<int>
+    reads this
+    requires isValid()
+  {
+    M.keys(entries)
+  }
 
   // this.valueSet() is the set of all the values in the map 
   ghost function valueSet(): set<T>
+    reads this
+    requires isValid()
+  {
+    M.values(entries)
+  }
 
   // A map m is valid iff it contains no repeated elements and
   // every key in m has exactly one associated value (no requires or ensures needed) 
-  ghost predicate isValid() 
+  ghost predicate isValid()
+    reads this
+  {
+    M.isValid(entries)
+  }
 
   // this.hasValue(k) is true iff key k as a value in the map
   ghost predicate hasValue(k: int)
+    reads this
+    requires isValid()
+  {
+    k in keySet()
+  }
 
   // this.isEmpty() is true iff the map contains no entries
-  predicate isEmpty() 
+  predicate isEmpty()
+    reads this
+    requires isValid()
+  {
+    entries == List.Nil
+  }
 
   // constructor returns a (new) map with an empty set of entries.
   constructor ()
+    ensures isValid()
+    ensures isEmpty()
+  {
+    entries := List.Nil;
+  }
 
   // this.size() returns the number of entries in the map
-  method size() returns (s: nat) 
+  method size() returns (s: nat)
+    requires isValid()
+    ensures s == |entrySet()|
+    ensures isValid()
+  {
+    s := M.size(entries);
+  }
 
   // this.get(k) returns the value associated to key k in the map, if any.
   // More precisely, it returns Some(v) if k has an associated value v,
   // and returns None otherwhise.
   method get(k: int) returns (vo: Option<T>)
-
+    requires isValid()
+    ensures k in keySet() ==> exists v :: vo == Some(v) && (k, v) in entrySet()
+    ensures k !in keySet() ==> vo == None
+    ensures isValid()
+  {
+    vo := M.get(entries, k);
+  }
   // this.put(k, v) changes the map so that key k is associated with value v.
   // Then it returns the value previously associated to k in the map, if any.
   // More precisely, it returns Some(v) if k had an associated value v,
   // and returns None otherwhise.
   method put(k: int, v: T) returns (old_vo: Option<T>)
-
+    modifies this
+    requires isValid()
+    ensures k in old(keySet()) ==> exists v' :: (k, v') in old(entrySet()) && entrySet() == (old(entrySet())) - {(k, v')} + {(k, v)}
+    ensures k !in old(keySet()) ==> entrySet() == old(entrySet()) + {(k, v)}
+    ensures isValid()
+  {
+    old_vo := get(k);
+    entries := M.put(entries, k, v);
+  }
   // this.remove(k) removes from the map the entry eith key k, if any.
   // Then it returns the value previously associated to k in the map, if any.
   // More precisely, it returns Some(v) if k had an associated value v,
   // and returns None otherwhise.
   method remove(k: int) returns (vo: Option<T>)
+    modifies this
+    requires isValid()
+    ensures k in old(keySet()) ==> exists v :: (k, v) in old(entrySet()) && entrySet() == old(entrySet()) - {(k, v)}
+    ensures k !in old(keySet()) ==> entrySet() == old(entrySet())
+    ensures isValid()
+  {
+    vo := get(k);
+    entries := M.remove(entries, k);
+  }
 }
